Spectre.thy
@@ -8,26 +8,126 @@ begin
 
 section  \<open>Spectre\<close>
  
-locale tie_breakingDAG = 
-  fixes G::"('a::linorder,'b) pre_digraph"
-  assumes is_blockDAG: "blockDAG G"
+locale tie_breakingDAG = blockDAG G for  
+   G::"('a::linorder,'b) pre_digraph"
+
 
 sublocale tie_breakingDAG \<subseteq> blockDAG using tie_breakingDAG_def tie_breakingDAG_axioms by auto 
 
 subsection  \<open>Functions and Definitions\<close>
+
+
+function genesis_nodeAlt:: "('a::linorder,'b) pre_digraph \<Rightarrow> 'a"
+  where "genesis_nodeAlt G = (if (\<not> blockDAG G) then undefined else 
+  if (card (verts G ) = 1) then (hd (sorted_list_of_set (verts G)))
+  else genesis_nodeAlt (reduce_past G ((hd (sorted_list_of_set (tips G))))))"
+  by auto 
+termination proof 
+  let ?R = "measure ( \<lambda>G. (card (verts G)))"
+  show "wf ?R" by auto
+next
+  fix G ::"('a::linorder,'b) pre_digraph"
+  assume "\<not> \<not> blockDAG G"
+  then have bD: "blockDAG G" by simp
+  assume "card (verts G) \<noteq> 1"
+  then have bG: "card (verts G) > 1" using bD blockDAG.blockDAG_size_cases by auto 
+  have " set (sorted_list_of_set (tips G)) = tips G"  
+    by (simp add: bD subs tips_def fin_digraph.finite_verts)
+  then have " hd (sorted_list_of_set (tips G)) \<in> tips G"  
+    using hd_in_set bD  tips_def bG blockDAG.tips_unequal_gen_exist 
+        empty_iff empty_set mem_Collect_eq
+    by (metis (mono_tags, lifting))  
+  then show "(reduce_past G (hd (sorted_list_of_set (tips G))), G) \<in> measure (\<lambda>G. card (verts G))"
+    using blockDAG.reduce_less bD
+    using tips_def by fastforce 
+qed
+
+lemma genesis_nodeAlt_one_sound:
+  assumes bD: "blockDAG G"
+  and one: "card (verts G) = 1"
+  shows "blockDAG.is_genesis_node G (genesis_nodeAlt G)" 
+proof -
+  have exone: "\<exists>! x. x \<in> (verts G)"
+    using bD one blockDAG.genesis_in_verts blockDAG.genesis_unique_exists blockDAG.reduce_less
+        blockDAG.reduce_past_dagbased less_nat_zero_code less_one by metis 
+  then have "sorted_list_of_set (verts G) \<noteq> []"
+    by (metis card.infinite card_0_eq finite.emptyI one 
+        sorted_list_of_set_empty sorted_list_of_set_inject zero_neq_one) 
+  then have "genesis_nodeAlt G \<in> verts G" using hd_in_set genesis_nodeAlt.simps bD exone
+    by (metis one set_sorted_list_of_set sorted_list_of_set.infinite) 
+  then show one_sound: "blockDAG.is_genesis_node G (genesis_nodeAlt G)"
+    using bD one 
+    by (metis blockDAG.blockDAG_size_cases blockDAG.reduce_less
+        blockDAG.reduce_past_dagbased less_one not_one_less_zero)
+qed
+
+lemma genesis_nodeAlt_sound : 
+  assumes "blockDAG G"
+  shows "blockDAG.is_genesis_node G (genesis_nodeAlt G)" 
+proof(induct_tac G rule:blockDAG_nat_less_induct)
+  show "blockDAG G" using assms by simp
+next 
+  fix V::"('a,'b) pre_digraph"
+  assume bD: "blockDAG V"
+  assume one: "card (verts V) = 1"
+  then show "blockDAG.is_genesis_node V (genesis_nodeAlt V)"
+    using genesis_nodeAlt_one_sound bD
+    by blast 
+next
+  fix W::"('a,'b) pre_digraph"
+  fix c::nat
+  assume basis: 
+    "(\<And>V::('a,'b) pre_digraph. blockDAG V \<Longrightarrow> card (verts V) < c \<Longrightarrow> 
+  blockDAG.is_genesis_node V (genesis_nodeAlt V))"
+  assume bD: "blockDAG W"
+  assume cd: "card (verts W) = c" 
+  consider (one) "card (verts W) = 1" | (more) "card (verts W) > 1"
+    using bD blockDAG.blockDAG_size_cases by blast
+  then show "blockDAG.is_genesis_node W (genesis_nodeAlt W)" 
+  proof(cases)
+    case one
+    then show ?thesis  using genesis_nodeAlt_one_sound bD
+    by blast
+  next
+    case more
+    then have not_one: "1 \<noteq> card (verts W)" by auto
+    have se: " set (sorted_list_of_set (tips W)) = tips W"  
+       by (simp add: bD subs  tips_def fin_digraph.finite_verts)
+     obtain a where a_def: "a = hd (sorted_list_of_set (tips W))"
+       by simp 
+    have tip: "a \<in> tips W"  
+    using se a_def hd_in_set bD  tips_def more  blockDAG.tips_unequal_gen_exist 
+        empty_iff empty_set mem_Collect_eq
+    by (metis (mono_tags, lifting))    
+    then have ver: "a \<in> verts W" 
+      by (simp add: tips_def a_def) 
+    then have "card ( verts (reduce_past W a)) < card (verts W)"
+      using more cd  blockDAG.reduce_less bD
+      by metis 
+    then have cd2: "card ( verts (reduce_past W a)) < c"
+      using cd by simp
+    have n_gen: "\<not> blockDAG.is_genesis_node W a"
+      using blockDAG.tips_unequal_gen bD more tip  tips_def Collect_mem_eq by fastforce
+    then have bD2: "blockDAG (reduce_past W a)"
+      using blockDAG.reduce_past_dagbased ver bD by auto
+    have ff: "blockDAG.is_genesis_node (reduce_past W a)
+     (genesis_nodeAlt (reduce_past W a))" using cd2 basis bD2 more
+      by blast
+    have rec: "genesis_nodeAlt W = genesis_nodeAlt (reduce_past W (hd (sorted_list_of_set (tips W))))"
+      using genesis_nodeAlt.simps not_one bD
+      by metis 
+    show ?thesis using rec ff bD n_gen ver blockDAG.reduce_past_gen_eq  a_def by metis
+  qed
+qed
 
 fun tie_break_int:: "'a::linorder \<Rightarrow> 'a \<Rightarrow> int \<Rightarrow> int"
   where "tie_break_int a b i =
  (if i=0 then (if (b < a) then -1 else 1) else 
               (if i > 0 then 1 else -1))"
 
-fun sumlist_break_acc :: "'a::linorder \<Rightarrow>'a \<Rightarrow> int \<Rightarrow> int list \<Rightarrow> int"
-  where "sumlist_break_acc a b s [] = tie_break_int a b s"
-  | "sumlist_break_acc a b s (x#xs) = sumlist_break_acc a b (s + x) xs"
-
 fun sumlist_break :: "'a::linorder \<Rightarrow>'a \<Rightarrow> int list \<Rightarrow> int"
-  where "sumlist_break a b [] = 0"
-  | "sumlist_break a b (x # xs) = sumlist_break_acc a b 0 (x # xs)"
+  where "sumlist_break a b [] = 0" (* votes like virtual block*)
+  | "sumlist_break a b (x # xs) = tie_break_int a b (sum_list (x # xs))"
 
 function vote_Spectre :: "('a::linorder,'b) pre_digraph \<Rightarrow>'a \<Rightarrow> 'a \<Rightarrow> 'a \<Rightarrow> int" 
   where
@@ -98,41 +198,52 @@ fun SpectreOrder :: "('a::linorder,'b) pre_digraph \<Rightarrow> 'a \<Rightarrow
   where "SpectreOrder G a b = ( sumlist_break a b (map (\<lambda>i.
    (vote_Spectre G i a b)) (sorted_list_of_set (verts G))) = 1)" 
 
+fun SpectreOrderAlt :: "('a::linorder,'b) pre_digraph \<Rightarrow> 'a \<Rightarrow> 'a \<Rightarrow> bool"
+  where "SpectreOrderAlt G a b = (if (\<not> blockDAG G) then undefined else
+ (vote_Spectre G (genesis_nodeAlt G) a b) = 1)" 
+
+
 subsubsection \<open>Lemmas\<close>
 
 lemma domain_tie_break:
-  shows "tie_break_int a b c \<in> {-1 ,0 ,1}"
+  shows "tie_break_int a b c \<in> {-1 ,1}"
   using  tie_break_int.simps by simp
-
-lemma domain_sumlist_acc:
-  shows "sumlist_break_acc a b c d \<in> {-1 ,0 ,1}"
-proof(induction d arbitrary: a b c)
-  case Nil
-  then show ?case by auto
-next
-  case (Cons d2 d)
-  then show ?case using Spectre.sumlist_break_acc.simps(2) by metis
-qed
 
 lemma domain_sumlist:
   shows "sumlist_break a b c  \<in> {-1 ,0 ,1}"
-  using domain_sumlist_acc sumlist_break.simps(1)
-  by (metis insertCI sumlist_break.elims) 
+  using sumlist_break.simps(1) insertCI sumlist_break.elims domain_tie_break
+  by (metis insert_commute)
+  
+   
+
+lemma domain_sumlist_not_empty:
+  assumes "l \<noteq> []"
+  shows "sumlist_break a b l  \<in> {-1, 1}"
+  using  sumlist_break.elims domain_tie_break assms
+  by metis 
+  
+  
 
 lemma Spectre_casesAlt:
   fixes V:: "('a::linorder,'b) pre_digraph"
-  and a :: "'a::linorder" and  b::  "'a::linorder" and c ::  "'a::linorder"
+  and a :: "'a::linorder" and  b :: "'a::linorder" and c :: "'a::linorder"
   obtains (no_bD) "(\<not> blockDAG V \<or> a \<notin> verts V \<or> b \<notin> verts V \<or> c \<notin> verts V)"
   | (equal) "(blockDAG V \<and> a \<in> verts V \<and> b \<in> verts V \<and> c \<in> verts V) \<and> b = c" 
   | (one) "(blockDAG V \<and> a \<in> verts V \<and> b \<in> verts V \<and> c \<in> verts V) \<and>
-         b \<noteq> c  \<and> ((a \<rightarrow>\<^sup>*\<^bsub>V\<^esub> b) \<and> \<not>(a \<rightarrow>\<^sup>*\<^bsub>V\<^esub> c))" 
-  | (two) "(blockDAG V \<and> a \<in> verts V \<and> b \<in> verts V \<and> c \<in> verts V) \<and> b \<noteq> c  \<and> 
-  \<not>((a \<rightarrow>\<^sup>*\<^bsub>V\<^esub> b) \<and> \<not>(a \<rightarrow>\<^sup>*\<^bsub>V\<^esub> c))\<and> ((a \<rightarrow>\<^sup>*\<^bsub>V\<^esub> c) \<and> \<not>(a \<rightarrow>\<^sup>*\<^bsub>V\<^esub> b))"
-  | (three) "(blockDAG V \<and> a \<in> verts V \<and> b \<in> verts V \<and> c \<in> verts V) \<and> b \<noteq> c  \<and> 
-  \<not>((a \<rightarrow>\<^sup>*\<^bsub>V\<^esub> b) \<and> \<not>(a \<rightarrow>\<^sup>*\<^bsub>V\<^esub> c))\<and> \<not>((a \<rightarrow>\<^sup>*\<^bsub>V\<^esub> c) \<and> \<not>(a \<rightarrow>\<^sup>*\<^bsub>V\<^esub> b)) \<and> ((a \<rightarrow>\<^sup>+\<^bsub>V\<^esub> b) \<and> (a \<rightarrow>\<^sup>+\<^bsub>V\<^esub> c))"
-  | (four) "(blockDAG V \<and> a \<in> verts V \<and> b \<in> verts V \<and> c \<in> verts V) \<and> b \<noteq> c  \<and> 
-  \<not>((a \<rightarrow>\<^sup>*\<^bsub>V\<^esub> b) \<and> \<not>(a \<rightarrow>\<^sup>*\<^bsub>V\<^esub> c))\<and> \<not>((a \<rightarrow>\<^sup>*\<^bsub>V\<^esub> c) \<and> \<not>(a \<rightarrow>\<^sup>*\<^bsub>V\<^esub> b)) \<and> \<not>((a \<rightarrow>\<^sup>+\<^bsub>V\<^esub> b) \<and> (a \<rightarrow>\<^sup>+\<^bsub>V\<^esub> c))"
+         b \<noteq> c  \<and> (((a \<rightarrow>\<^sup>+\<^bsub>V\<^esub> b) \<or> a = b) \<and> \<not>(a \<rightarrow>\<^sup>+\<^bsub>V\<^esub> c))" 
+  | (two) "(blockDAG V \<and> a \<in> verts V \<and> b \<in> verts V \<and> c \<in> verts V) \<and> b \<noteq> c 
+  \<and> \<not>(((a \<rightarrow>\<^sup>+\<^bsub>V\<^esub> b) \<or> a = b) \<and> \<not>(a \<rightarrow>\<^sup>+\<^bsub>V\<^esub> c)) \<and> 
+  ((a \<rightarrow>\<^sup>+\<^bsub>V\<^esub> c) \<or> a = c) \<and> \<not>(a \<rightarrow>\<^sup>+\<^bsub>V\<^esub> b)"
+  | (three) "(blockDAG V \<and> a \<in> verts V \<and> b \<in> verts V \<and> c \<in> verts V) \<and> b \<noteq> c 
+   \<and> \<not>(((a \<rightarrow>\<^sup>+\<^bsub>V\<^esub> b) \<or> a = b) \<and> \<not>(a \<rightarrow>\<^sup>+\<^bsub>V\<^esub> c)) \<and>  
+   \<not>(((a \<rightarrow>\<^sup>+\<^bsub>V\<^esub> c) \<or> a = c) \<and> \<not>(a \<rightarrow>\<^sup>+\<^bsub>V\<^esub> b))\<and> 
+  ((a \<rightarrow>\<^sup>+\<^bsub>V\<^esub> b) \<and> (a \<rightarrow>\<^sup>+\<^bsub>V\<^esub> c))"
+  | (four) "(blockDAG V \<and> a \<in> verts V \<and> b \<in> verts V \<and> c \<in> verts V) \<and> b \<noteq> c  \<and>
+  \<not>(((a \<rightarrow>\<^sup>+\<^bsub>V\<^esub> b) \<or> a = b) \<and> \<not>(a \<rightarrow>\<^sup>+\<^bsub>V\<^esub> c)) \<and>  
+   \<not>(((a \<rightarrow>\<^sup>+\<^bsub>V\<^esub> c) \<or> a = c) \<and> \<not>(a \<rightarrow>\<^sup>+\<^bsub>V\<^esub> b))\<and>  
+  \<not>((a \<rightarrow>\<^sup>+\<^bsub>V\<^esub> b) \<and> (a \<rightarrow>\<^sup>+\<^bsub>V\<^esub> c))"
   by auto
+  
 
 lemma Spectre_theo:
   assumes "P 0"
@@ -162,54 +273,167 @@ qed
 
 
 lemma antisymmetric_tie_break:
-  shows "b\<noteq>c \<and> i = 0 \<Longrightarrow> tie_break_int b c i = - tie_break_int c b i"
+  shows "b\<noteq>c  \<Longrightarrow> tie_break_int b c i = - tie_break_int c b (-i)"
   unfolding  tie_break_int.simps using less_not_sym by auto
 
-
-lemma antisymmetric_sumlist_acc:
-  shows "b \<noteq> c  \<Longrightarrow> sumlist_break_acc b c s l1 = - sumlist_break_acc c b (-s) ( map (\<lambda>x. -x) l1)"
-proof(induction l1 arbitrary:  b c s)
+   
+lemma antisymmetric_sumlist:
+  shows "b \<noteq> c \<Longrightarrow> sumlist_break b c l = - sumlist_break c b (map (\<lambda>x. -x) l) "
+proof(induct l)
   case Nil
-  then show ?case using sumlist_break_acc.simps(1) antisymmetric_tie_break by auto
+  then show ?case by simp
 next
   case (Cons a l)
-  then show ?case unfolding list.simps(9) sumlist_break_acc.simps(2) by auto  
+  have "sum_list (map uminus (a # l)) = - sum_list  (a # l)"
+    by (metis map_ident map_map uminus_sum_list_map) 
+  then show ?case using sumlist_break.simps(2) antisymmetric_tie_break Cons by auto
 qed
   
 
-lemma antisymmetric_sumlist:
-  shows "b \<noteq> c \<Longrightarrow> sumlist_break b c l = - sumlist_break c b (map (\<lambda>x. -x) l) "
-  using antisymmetric_sumlist_acc sumlist_break.simps(2) by (cases l) auto
 
-
-lemma Spectre_antisymmetric: 
-  shows "\<And> V a b c.  b \<noteq> c \<longrightarrow> vote_Spectre V a b c = - vote_Spectre V a c b"
-proof -
+lemma vote_Spectre_antisymmetric: 
+  shows "b \<noteq> c \<Longrightarrow> vote_Spectre V a b c = - (vote_Spectre V a c b)"
+proof(induction V a b c rule: vote_Spectre.induct)
   fix V ::"('a::linorder, 'b) pre_digraph"
-  fix a b c
-  consider (nbD) "(\<not> blockDAG V \<or> a \<notin> verts V \<or> b \<notin> verts V \<or> c \<notin> verts V)" 
-    | (bD) "\<not>(\<not> blockDAG V \<or> a \<notin> verts V \<or> b \<notin> verts V \<or> c \<notin> verts V)" by auto
-  then show "b \<noteq> c \<longrightarrow> vote_Spectre V a b c = - vote_Spectre V a c b"
-  proof( cases)
-    case nbD
+  and a:: "'a::linorder" and  b:: "'a::linorder" and  c :: "'a::linorder"
+  assume past: "(\<And>x. \<not> (\<not> blockDAG V \<or> a \<notin> verts V \<or> b \<notin> verts V \<or> c \<notin> verts V) \<Longrightarrow>
+             b \<noteq> c \<Longrightarrow>
+             \<not> ((a \<rightarrow>\<^sup>+\<^bsub>V\<^esub> b \<or> a = b) \<and> (a, c) \<notin> (arcs_ends V)\<^sup>+) \<Longrightarrow>
+             \<not> ((a \<rightarrow>\<^sup>+\<^bsub>V\<^esub> c \<or> a = c) \<and> (a, b) \<notin> (arcs_ends V)\<^sup>+) \<Longrightarrow>
+             a \<rightarrow>\<^sup>+\<^bsub>V\<^esub> b \<and> a \<rightarrow>\<^sup>+\<^bsub>V\<^esub> c \<Longrightarrow>
+             x \<in> set (sorted_list_of_set (past_nodes V a)) \<Longrightarrow>
+              b \<noteq> c \<Longrightarrow> vote_Spectre (reduce_past V a) x b c
+               = - vote_Spectre (reduce_past V a) x c b)"
+  and fut: "(\<And>x. \<not> (\<not> blockDAG V \<or> a \<notin> verts V \<or> b \<notin> verts V \<or> c \<notin> verts V) \<Longrightarrow>
+             b \<noteq> c \<Longrightarrow>
+             \<not> ((a \<rightarrow>\<^sup>+\<^bsub>V\<^esub> b \<or> a = b) \<and> (a, c) \<notin> (arcs_ends V)\<^sup>+) \<Longrightarrow>
+             \<not> ((a \<rightarrow>\<^sup>+\<^bsub>V\<^esub> c \<or> a = c) \<and> (a, b) \<notin> (arcs_ends V)\<^sup>+) \<Longrightarrow>
+             \<not> (a \<rightarrow>\<^sup>+\<^bsub>V\<^esub> b \<and> a \<rightarrow>\<^sup>+\<^bsub>V\<^esub> c) \<Longrightarrow>
+             x \<in> set (sorted_list_of_set (future_nodes V a)) \<Longrightarrow>
+             b \<noteq> c \<Longrightarrow> vote_Spectre V x b c = - vote_Spectre V x c b)"
+  and not_eq: "b \<noteq> c"
+  show "vote_Spectre V a b c = - vote_Spectre V a c b"
+  proof(cases a b c V rule:Spectre_casesAlt)
+  case no_bD
     then show ?thesis by auto
   next
-    case bD
-    then have "blockDAG V" by auto
-    then show ?thesis using bD
-    proof(induction V rule:blockDAG_nat_less_induct)
-      case (base V)
-      then have "verts V = {blockDAG.genesis_node V}" 
-        using blockDAG.gen_gen blockDAG.gen_graph_all_one
-        by metis 
-      then show ?case by auto 
-    next
-      case (step V)
-      then show ?case 
-     
-                                 
-lemma (in tie_breakingDAG) "total_on (verts G) SpectreOrder"
-  unfolding total_on_def SpectreOrder 
+  case equal
+  then show ?thesis using not_eq  by simp
+  next
+    case one
+    then show ?thesis by auto   
+  next
+    case two
+    then show ?thesis by auto
+  next
+    case three
+    then have ff: "vote_Spectre V a b c = (sumlist_break b c (map (\<lambda>i.
+ (vote_Spectre (reduce_past V a) i b c)) (sorted_list_of_set (past_nodes V a))))" by auto
+    have ff2: "vote_Spectre V a c b = (sumlist_break c b (map (\<lambda>i.
+    (- vote_Spectre (reduce_past V a) i b c)) (sorted_list_of_set (past_nodes V a))))" 
+       using three past vote_Spectre.simps map_eq_conv
+       by (smt (verit))
+     have "(map (\<lambda>i. - vote_Spectre (reduce_past V a) i b c) (sorted_list_of_set (past_nodes V a)))
+     = (map uminus (map (\<lambda>i. vote_Spectre (reduce_past V a) i b c)
+       (sorted_list_of_set (past_nodes V a))))" 
+       using map_map by auto       
+     then have "vote_Spectre V a c b = - (sumlist_break b c (map (\<lambda>i.
+    (vote_Spectre (reduce_past V a) i b c)) (sorted_list_of_set (past_nodes V a))))" 
+    using  antisymmetric_sumlist not_eq ff2
+    by (metis verit_minus_simplify(4)) 
+    then show ?thesis using  ff by auto
+  next
+    case four
+    then have ff: "vote_Spectre V a b c = sumlist_break b c (map (\<lambda>i.
+   (vote_Spectre V i b c)) (sorted_list_of_set (future_nodes V a)))" by auto 
+    have ff2: "vote_Spectre V a c b = (sumlist_break c b (map (\<lambda>i.
+    (- vote_Spectre V i b c)) (sorted_list_of_set (future_nodes V a))))" 
+       using four fut vote_Spectre.simps map_eq_conv
+       by (smt (z3))
+     have "(map (\<lambda>i. - vote_Spectre V i b c) (sorted_list_of_set (future_nodes V a)))
+     = (map uminus (map (\<lambda>i. vote_Spectre V i b c) (sorted_list_of_set (future_nodes V a))))" 
+       using map_map by auto       
+     then have "vote_Spectre V a c b = - (sumlist_break b c (map (\<lambda>i.
+    (vote_Spectre V i b c)) (sorted_list_of_set (future_nodes V a))))" 
+    using  antisymmetric_sumlist not_eq ff2
+    by (metis verit_minus_simplify(4)) 
+    then show ?thesis using ff by auto
+  qed  
+qed
+
+
+lemma vote_Spectre_reflexiv:
+assumes "blockDAG V"
+  and "a \<in> verts V"
+shows "\<forall>b \<in> verts V. vote_Spectre V b a a = 1 " using vote_Spectre.simps assms by auto 
+
+lemma SpectreOrder_reflexiv:
+assumes "blockDAG V"
+  and "a \<in> verts V" 
+shows "SpectreOrder V a a" 
+  unfolding SpectreOrder.simps 
+proof -   
+  obtain l where l_def: "l = (map (\<lambda>i. vote_Spectre V i a a) (sorted_list_of_set (verts V)))"
+    by auto
+  have only_one: "l = (map (\<lambda>i.1) (sorted_list_of_set (verts V)))"
+    using l_def vote_Spectre_reflexiv assms sorted_list_of_set(1)
+    by (simp add: fin_digraph.finite_verts subs)
+  have ne: "l \<noteq> []"
+    using  blockDAG.no_empty_blockDAG length_map
+    by (metis assms(1) length_sorted_list_of_set less_numeral_extra(3) list.size(3) l_def)
+  have "sum_list l = card (verts V)" using ne only_one sum_list_map_eq_sum_count
+    by (simp add: sum_list_triv)
+  then have "sum_list l > 0" using blockDAG.no_empty_blockDAG assms(1) by simp
+  then show "sumlist_break a a (map (\<lambda>i. vote_Spectre V i a a) (sorted_list_of_set (verts V))) = 1"
+    using l_def ne sumlist_break.simps(2) tie_break_int.simps
+    by (metis list.exhaust verit_comp_simplify1(1)) 
+qed
+
+lemma Spectre_Order_antisymmetric: 
+  assumes "blockDAG V"
+  and "a \<in> verts V \<and> b \<in> verts V" 
+  and "a \<noteq> b"
+  shows "SpectreOrder V a b = (\<not> (SpectreOrder V b a))"
+proof -
+  obtain l where l_def: "l = (map (\<lambda>i. vote_Spectre V i a b) (sorted_list_of_set (verts V)))"
+    by auto
+  then have ne: "l \<noteq> []"
+    using  blockDAG.no_empty_blockDAG length_map assms(1)
+      length_sorted_list_of_set less_numeral_extra(3) list.size(3) l_def
+    by metis
+  then have dm: "sumlist_break a b l \<in> {-1,1}" using domain_sumlist_not_empty by auto  
+  obtain l2 where l2_def: "l2 = (map (\<lambda>i. vote_Spectre V i b a) (sorted_list_of_set (verts V)))"
+      by auto
+    have minus: "l2 = map uminus l"
+      unfolding l_def l2_def map_map
+      using  vote_Spectre_antisymmetric assms(3)
+      by (metis comp_apply) 
+    have anti: "sumlist_break a b l = - sumlist_break b a l2" unfolding minus 
+      using antisymmetric_sumlist assms(3) by auto
+    have ne2: "l2 \<noteq> []"
+      using ne minus by auto
+    then have dm2: "sumlist_break b a l2 \<in> {-1,1}" using domain_sumlist_not_empty by auto
+    then show "?thesis" unfolding SpectreOrder.simps using anti l_def dm l2_def 
+    add.inverse_inverse empty_iff equal_neg_zero insert_iff zero_neq_one
+    by (metis)
+qed  
   
+lemma SpectreOrder_total:
+  assumes "blockDAG V"
+  and "a \<in> verts V \<and> b \<in> verts V" 
+shows "SpectreOrder V a b \<or> SpectreOrder V b a"
+proof safe
+  assume notB: " \<not> SpectreOrder V b a"
+  consider (eq) "a = b"| (neq) "a \<noteq> b" by auto
+  then show "SpectreOrder V a b"
+  proof (cases)
+  case eq
+  then show ?thesis using SpectreOrder_reflexiv assms by metis
+  next
+    case neq
+     then show "?thesis" using Spectre_Order_antisymmetric notB assms
+       by blast 
+   qed
+ qed
 
 end
